deps/poulet4/lib/P4automata/Examples/BabyIP.v
@@ -78,9 +78,7 @@ Module BabyIP1.
 
   Program Definition aut: Syntax.t state header :=
     {| t_states := states |}.
-  Next Obligation.
-    destruct s; cbv; Lia.lia.
-  Qed.
+  Solve Obligations with (destruct s; cbv; Lia.lia).
 
 End BabyIP1.
 
@@ -145,9 +143,7 @@ Module BabyIP2.
 
   Program Definition aut: Syntax.t state header :=
     {| t_states := states |}.
-  Next Obligation.
-    destruct s; cbv; Lia.lia.
-  Qed.
+  Solve Obligations with (destruct s; cbv; Lia.lia).
 
 End BabyIP2.
 
